added adequacy proof to CSem

coq/CSem.v
@@ -1,20 +1,53 @@
-(** * Concrete Execution Semantics *)
+(** * Concrete Execution Semantics
 
-Require Import FunInd ListSet Arith Program Lia.
+    This library presents a message algebra, called the concrete
+    message algebra, that is very similar to the algebra used by the
+    abstract execution semantics.  The only difference is the way in
+    which it models encryption.  The signature used by the previous
+    algebra has a binary operator for encryption [En], which suggests
+    that two encryptions are the same if the plaintext and the key
+    used to construct them are the same.  This is not true for
+    implementations of encryption in actual use.  Instead, some
+    randomness is added to an encryption during its construction in
+    such a way that knowledge of the randomness is not needed to
+    recover the plaintext by someone in possession of the decryption
+    key.
+
+    Probabilistic encryption is modeled by adding a random natural
+    number to the construction of every term that represents an
+    encryption.  A semantics is defined around the new algebra.  The
+    new semantics is shown to be faithful to the abstract execution
+    semantics, that is, for every run of the concrete execution
+    semantics, there is a corresponding run of the abstract semantics
+    in Theorem [csem_sem_faithfulness].  The concrete semantics is
+    shown to be adequate with respect to the abstract execution
+    semantics, that is for every run of the abstract execution
+    semantics and choice of random values, there is a run of the
+    concrete execution semantics, in Theorem [sem_csem_adequacy].
+
+    The proof of adequacy makes demands on both the abstract and
+    concrete execution semantics.  The proof depends on the fact that
+    the following terms may not contain an encryption,
+
+    - the key used during a decryption,
+
+    - the terms compared with a sameness check, and
+
+    - the terms compared with an inverse key predicate check. *)
+
+Require Import FunInd ListSet Bool Arith Program Lia.
 Require Import Preamble Monad Proc Alg Sem.
 Import List.ListNotations.
 Open Scope list_scope.
 
-(** Concrete message algebra
+(** ** Definition and Faithfulness
 
-    Notice that encryptions take one more argument as compared with
-    encryptions in the message algebra.  The extra argument is some
-    randomness.  See [CEn].  This is how probabilistic encryption is
-    modeled.
+    The key theorem in this section is [csem_sem_faithfulness], which
+    states that whenever there is a run in the concrete executions
+    semantics, there is a corresponding run in the abstract execution
+    semantics.
 
-    The key theorem in this library is [csem_sem], which states that
-    whenever there is a run in the concrete executions semantics,
-    there is a corresponding run in the abstract execution semantics. *)
+    Concrete message algebra *)
 
 Inductive calg: Set :=
 | CTx: var -> calg              (* Text *)
@@ -31,6 +64,11 @@ Inductive calg: Set :=
 | CHs: calg -> calg.            (* Hash *)
 
 (* An uninformative comment added to make coqdoc happy *)
+
+(** Notice that encryptions take one more argument as compared with
+    encryptions in the abstract message algebra.  The extra argument
+    is some randomness.  See [CEn].  This is how probabilistic
+    encryption is modeled. *)
 
 Definition calg_dec:
   forall x y: calg, {x = y} + {x <> y}.
@@ -77,6 +115,14 @@ Proof.
   destruct c; simpl; auto.
 Qed.
 
+Fixpoint chas_enc (x: calg): bool :=
+  match x with
+  | CHs y => chas_enc y
+  | CPr y z => chas_enc y || chas_enc z
+  | CEn _ _ _ => true
+  | _ => false
+  end.
+
 (** Convert an concrete message [x] into its equivalent message.  This
     is done by forgetting the randomness in each encryption. *)
 
@@ -95,6 +141,40 @@ Fixpoint to_alg (x: calg): alg :=
   | CEn _ y z => En (to_alg y) (to_alg z)
   | CHs y => Hs (to_alg y)
   end.
+
+Lemma inv_to_alg:
+  forall x,
+    inv (to_alg x) = to_alg (cinv x).
+Proof.
+  intros.
+  destruct x; simpl; auto.
+Qed.
+
+Lemma no_enc_eq:
+  forall x y,
+    chas_enc x = false ->
+    to_alg x = to_alg y ->
+    x = y.
+Proof.
+  induction x; induction y; intros;
+    simpl in H; simpl in H0; inv H0; auto.
+  - rewrite orb_false_iff in H.
+    destruct H.
+    apply IHx1 in H2; auto.
+    apply IHx2 in H3; auto; subst; auto.
+  - inv H.
+  - apply IHx in H2; subst; auto.
+Qed.
+
+Lemma has_enc_to_alg:
+  forall x,
+    chas_enc x = has_enc (to_alg x).
+Proof.
+  induction x; intros; simpl; auto.
+  rewrite IHx1.
+  rewrite IHx2.
+  auto.
+Qed.
 
 (** Convert a concrete event *)
 
@@ -164,14 +244,6 @@ Proof.
     destruct c2; inv H3; auto.
 Qed.
 
-Lemma inv_to_alg:
-  forall x,
-    inv (to_alg x) = to_alg (cinv x).
-Proof.
-  intros.
-  destruct x; simpl; auto.
-Qed.
-
 (** The semantics of an expression
 
 <<
@@ -218,6 +290,7 @@ Inductive expr_csem: cenv -> list cevt -> list calg -> list nat ->
 | CExpr_decr: forall ev tr us rs x y r a b,
     lookup x ev = Some (CEn r a b) ->
     lookup y ev = Some (cinv b) ->
+    chas_enc (cinv b) = false ->
     expr_csem ev tr us rs (Decr_ x y) a tr us rs
 | CExpr_frsh: forall ev tr us rs a,
     expr_csem ev tr (a :: us) rs Frsh_ a tr us rs
@@ -260,6 +333,8 @@ Proof.
   intros.
   inv H; simpl; auto; lookup_and_type_check; eauto.
   rewrite <- inv_to_alg in H1.
+  rewrite has_enc_to_alg in H2.
+  rewrite <- inv_to_alg in H2.
   eauto.
 Qed.
 
@@ -293,11 +368,19 @@ Inductive stmt_csem: cenv -> list cevt -> list calg ->
 | CStmt_same: forall ev tr us rs x y a b,
     lookup x ev = Some a ->
     lookup y ev = Some b ->
+    chas_enc a = false ->       (* For probabilistic encryption *)
     a = b ->                    (* Sameness check *)
     stmt_csem ev tr us rs (Same x y) ev tr us rs
+| CStmt_ltkp: forall ev tr us rs x y z a b c,
+    lookup x ev = Some a ->
+    lookup y ev = Some (CNm b) ->
+    lookup z ev = Some (CNm c) ->
+    a = CSk (Lt b c) ->         (* Ltk check *)
+    stmt_csem ev tr us rs (Ltkp x y z) ev tr us rs
 | CStmt_invp: forall ev tr us rs x y a b,
     lookup x ev = Some a ->
     lookup y ev = Some b ->
+    chas_enc a = false ->       (* For probabilistic encryption *)
     a = cinv b ->               (* Inverse check *)
     stmt_csem ev tr us rs (Invp x y) ev tr us rs
 | CStmt_pub_namp: forall ev tr us rs x y a b,
@@ -340,6 +423,7 @@ Proof.
   - exists []; auto.
   - exists []; auto.
   - exists []; auto.
+  - exists []; auto.
 Qed.
 
 (** Main theorem about statements *)
@@ -355,14 +439,17 @@ Proof.
   - apply expr_csem_expr_sem in H0.
     apply Stmt_bind; auto.
   - apply Stmt_send; auto.
-  - eapply Stmt_invp; eauto.
+  - rewrite has_enc_to_alg in H2.
+    eapply Stmt_same; eauto.
+  - rewrite has_enc_to_alg in H2.
+    eapply Stmt_invp; eauto.
     rewrite inv_to_alg; auto.
 Qed.
 
 (** The semantics of a statement list
 
     Parameters as for [stmt_csem] but with one extra argument,
-    for outputs.
+    for outputs, and no output trace and list of uniques.
 
 <<
    Parameters:
@@ -374,28 +461,26 @@ Qed.
    stmts:     Statements
    cenv:      Output environment
    list cevt: Output trace
-   list calg: Output list of uniques
-   list nat:  Output list of random values
 >>
  *)
 
-Inductive stmt_list_csem: cenv -> list cevt -> list calg ->
-                          list nat -> list calg -> list stmt -> cenv ->
-                          list cevt -> list calg -> list nat -> Prop :=
+Inductive stmt_list_csem:
+  cenv -> list cevt -> list calg -> list nat ->
+  list calg -> list stmt -> cenv -> list nat -> Prop :=
 | CStmt_return: forall ev rs outs vs,
     map_m (flip lookup ev) vs = Some outs ->
-    stmt_list_csem ev [] [] rs outs [Return vs] ev [] [] rs
-| CStmt_pair: forall ev tr us rs outs stmt ev' tr' us' rs'
-                     stmts ev'' tr'' us'' rs'',
+    stmt_list_csem ev [] [] rs outs [Return vs] ev rs
+| CStmt_pair: forall ev tr us rs stmt ev' tr' us' rs'
+                     outs stmts ev'' rs'',
     stmt_csem ev tr us rs stmt ev' tr' us' rs' ->
-    stmt_list_csem ev' tr' us' rs' outs stmts ev'' tr'' us'' rs'' ->
-    stmt_list_csem ev tr us rs outs (stmt :: stmts) ev'' tr'' us'' rs''.
+    stmt_list_csem ev' tr' us' rs' outs stmts ev'' rs'' ->
+    stmt_list_csem ev tr us rs outs (stmt :: stmts) ev'' rs''.
 #[global]
 Hint Constructors stmt_list_csem : core.
 
 Lemma stmt_list_csem_env_extends:
-  forall ev tr us rs outs stmts ev' tr' us' rs',
-    stmt_list_csem ev tr us rs outs stmts ev' tr' us' rs' ->
+  forall ev tr us rs outs stmts ev' rs',
+    stmt_list_csem ev tr us rs outs stmts ev' rs' ->
     exists ev'', ev' = ev'' ++ ev.
 Proof.
   intros.
@@ -447,9 +532,9 @@ Qed.
 
 Theorem stmt_list_csem_stmt_list_sem:
   forall ev tr us rs outs stmts ev' rs',
-      stmt_list_csem ev tr us rs outs stmts ev' [] [] rs' ->
+      stmt_list_csem ev tr us rs outs stmts ev' rs' ->
       stmt_list_sem (to_env ev) (map to_evt tr) (map to_alg us)
-                    (map to_alg outs) stmts (to_env ev') [] [].
+                    (map to_alg outs) stmts (to_env ev').
 Proof.
   intros.
   induction H; simpl; auto.
@@ -504,14 +589,14 @@ Definition csem (p: proc) (rs: list nat) (cev: cenv) (e: role): Prop :=
     cins_inputs (ins p) cins /\
     exists ctr cus couts rs',
       let ev_in := mk_cenv (ins p) cins in
-      stmt_list_csem ev_in ctr cus rs couts (body p) cev [] [] rs' /\
+      stmt_list_csem ev_in ctr cus rs couts (body p) cev rs' /\
       trace e = map to_evt ctr /\
       uniqs e = map to_alg cus /\
       outputs e = map to_alg couts.
 
 (** Main theorem about the concrete semantics *)
 
-Theorem csem_sem:
+Theorem csem_sem_faithfulness:
   forall p rs cev e,
     csem p rs cev e -> sem p (to_env cev) e.
 Proof.
@@ -535,7 +620,1195 @@ Proof.
   split; auto.
 Qed.
 
-(** * Alternate Concrete Execution Semantics
+(** ** Adequacy
+
+    Theorem [sem_csem_adequacy] states that whenever there is a run of
+    the abstract semantics, there is a run of the concrete semantics.
+    The proof of this theorem is much more difficult than the proof of
+    the faithfulness theorem.  For that theorem, it is easy to create
+    a witness by simply eliminating randomness using the [to_alg]
+    function.  This section defines some simulation relations that
+    help find the correct witness. *)
+
+Lemma ex_lookup:
+  forall v ev a,
+    lookup v (to_env ev) = Some a ->
+    exists b, lookup v ev = Some b.
+Proof.
+  induction ev; intros; simpl in *; auto.
+  - inv H.
+  - unfold to_maplet in H.
+    repeat expand_let_pairs; simpl in *.
+    destruct (alt_bool_dec (fst a =? v)) as [G|G];
+      rewrite G in *.
+    + inv H.
+      destruct a as [u c]; simpl.
+      exists c; auto.
+    + eapply IHev; eauto.
+Qed.
+
+(** This theorem states that whenever an abstract expression has a
+    value, there is corresponding value in the concrete semantics.
+    The proof of this theorem depends on the fact that the key in a
+    decryption must not contain an encryption, and therefore, no
+    randomness.  See [CExpr_decr]. *)
+
+Theorem expr_sem_expr_csem:
+  forall ev tr us rs exp val tr' us' cev ctr cus,
+    expr_sem ev tr us exp val tr' us' ->
+    to_env cev = ev ->
+    map to_evt ctr = tr ->
+    map to_alg cus = us ->
+    exists cval ctr' cus' rs',
+      expr_csem cev ctr cus rs exp cval ctr' cus' rs' /\
+      to_alg cval = val /\
+      map to_evt ctr' = tr' /\
+      map to_alg cus' = us'.
+Proof.
+  intros.
+  destruct exp; inv H.
+  - exists (CTg s).
+    exists ctr.
+    exists cus.
+    exists rs.
+    simpl.
+    auto.
+  - pose proof H7 as G.
+    apply ex_lookup in H7.
+    destruct H7.
+    erewrite lookup_ev in G; eauto.
+    inv G; subst.
+    exists (CHs x).
+    repeat eexists.
+    apply CExpr_hash; auto.
+  - pose proof H8 as H.
+    apply ex_lookup in H8.
+    destruct H8.
+    erewrite lookup_ev in H; eauto.
+    inv H; subst.
+    pose proof H12 as H.
+    apply ex_lookup in H12.
+    destruct H12.
+    erewrite lookup_ev in H; eauto.
+    inv H; subst.
+    exists (CPr x x0); simpl.
+    repeat eexists; eauto.
+  - pose proof H8 as H.
+    apply ex_lookup in H8.
+    destruct H8.
+    erewrite lookup_ev in H; eauto.
+    inv H; subst.
+    pose proof H12 as H.
+    apply ex_lookup in H12.
+    destruct H12.
+    erewrite lookup_ev in H; eauto.
+    inv H; subst.
+    destruct rs as [|r rs].
+    + exists (CEn 0 x x0); simpl.
+      repeat eexists; eauto.
+    + exists (CEn r x x0); simpl.
+      repeat eexists; eauto.
+  - pose proof H7 as H.
+    apply ex_lookup in H7.
+    destruct H7.
+    erewrite lookup_ev in H; eauto.
+    inv H.
+    destruct x; simpl in H2; inv H2.
+    exists x1.
+    repeat eexists; eauto.
+  - pose proof H7 as H.
+    apply ex_lookup in H7.
+    destruct H7.
+    erewrite lookup_ev in H; eauto.
+    inv H.
+    destruct x; simpl in H2; inv H2.
+    exists x2.
+    repeat eexists; eauto.
+  - pose proof H5 as H.
+    apply ex_lookup in H5.
+    destruct H5.
+    erewrite lookup_ev in H; eauto.
+    inv H.
+    destruct x; simpl in H2; inv H2.
+    rewrite inv_to_alg in H13.
+    rewrite inv_to_alg in H9.
+    pose proof H9 as H.
+    apply ex_lookup in H9.
+    destruct H9.
+    erewrite lookup_ev in H; eauto.
+    inv H.
+    exists x1.
+    repeat eexists; eauto.
+    rewrite <- has_enc_to_alg in H13.
+    eapply CExpr_decr; eauto.
+    rewrite H1.
+    apply eq_sym in H3.
+    apply no_enc_eq in H3; subst; auto.
+  - destruct cus as [| u cus]; simpl in H5; inv H5.
+    exists u.
+    repeat eexists; eauto.
+  - destruct ctr as [| e ctr]; simpl in H5; inv H5.
+    destruct e; simpl in H0; inv H0.
+    pose proof H7 as H.
+    apply ex_lookup in H7.
+    destruct H7.
+    erewrite lookup_ev in H; eauto.
+    inv H.
+    destruct x; simpl in H2; inv H2.
+    exists c.
+    repeat eexists; eauto.
+Qed.
+
+(** The [stmt_send] conditions ensures that a transmitted message
+    agrees with what is in the environment. *)
+
+Definition stmt_send (ev: cenv) (ctr: list cevt) (s: stmt): Prop :=
+  match s, ctr with
+  | Send c x, CSd d a :: _ =>
+    lookup x ev = Some a
+  | _, _ => True
+  end.
+
+(** This theorem states that whenever an abstract state transitions,
+    there is corresponding transition in the concrete semantics.  The
+    proof of this theorem depends on the fact that the sameness and
+    inverse predicate checks never succeed when given a term that
+    contains an encryption, so checked terms contain no randomness.
+    See [CStmt_same] and [CStmt_invp]. *)
+
+Theorem stmt_sem_stmt_csem:
+  forall ev tr us cev ctr cus rs stmt ev' tr' us',
+    stmt_sem ev tr us stmt ev' tr' us' ->
+    to_env cev = ev ->
+    map to_evt ctr = tr ->
+    map to_alg cus = us ->
+    stmt_send cev ctr stmt ->
+    exists cev' ctr' cus' rs',
+      stmt_csem cev ctr cus rs stmt cev' ctr' cus' rs' /\
+      to_env cev' = ev' /\
+      map to_evt ctr' = tr' /\
+      map to_alg cus' = us'.
+Proof.
+  intros.
+  destruct stmt; inv H.
+  - apply expr_sem_expr_csem
+      with (rs := rs)
+           (cev := cev)
+           (ctr := ctr)
+           (cus := cus)
+      in H9; auto.
+    repeat destruct_ex_and; subst.
+    rewrite <- type_check_equiv in H13.
+    exists ((v, x) :: cev).
+    exists x0.
+    exists x1.
+    exists x2.
+    auto.
+  - destruct ctr as [|e ctr].
+    simpl in H7.
+    inv H7.
+    destruct e; simpl in H7; inv H7.
+    pose proof H9 as H.
+    apply ex_lookup in H9.
+    destruct H9.
+    erewrite lookup_ev in H; eauto.
+    inv H.
+    destruct x; simpl in H2; inv H2.
+    pose proof H13 as H.
+    apply ex_lookup in H13.
+    destruct H13.
+    erewrite lookup_ev in H; eauto.
+    inv H.
+    unfold stmt_send in H3.
+    rewrite H1 in H3.
+    inv H3.
+    repeat eexists; eauto.
+  - exists cev.
+    exists ctr.
+    exists cus.
+    exists rs.
+    pose proof H6 as H.
+    apply ex_lookup in H6.
+    destruct H6.
+    erewrite lookup_ev in H; eauto.
+    inv H.
+    pose proof H7 as H.
+    apply ex_lookup in H7.
+    destruct H7.
+    erewrite lookup_ev in H; eauto.
+    inv H.
+    rewrite <- has_enc_to_alg in H11; auto.
+    apply eq_sym in H4.
+    apply no_enc_eq in H4; auto; subst.
+    split; auto.
+    eapply CStmt_same; eauto.
+  - exists cev.
+    exists ctr.
+    exists cus.
+    exists rs.
+    pose proof H7 as H.
+    apply ex_lookup in H7.
+    destruct H7.
+    erewrite lookup_ev in H; eauto.
+    inv H.
+    destruct x; simpl in H2; inv H2.
+    pose proof H11 as H.
+    apply ex_lookup in H11.
+    destruct H11.
+    erewrite lookup_ev in H; eauto.
+    inv H.
+    destruct x; simpl in H4; inv H4.
+    pose proof H15 as H.
+    apply ex_lookup in H15.
+    destruct H15.
+    erewrite lookup_ev in H; eauto.
+    inv H.
+    destruct x; simpl in H5; inv H5.
+    split; auto.
+    eapply CStmt_ltkp; eauto.
+  - exists cev.
+    exists ctr.
+    exists cus.
+    exists rs.
+    pose proof H6 as H.
+    apply ex_lookup in H6.
+    destruct H6.
+    erewrite lookup_ev in H; eauto.
+    inv H.
+    pose proof H7 as H.
+    apply ex_lookup in H7.
+    destruct H7.
+    erewrite lookup_ev in H; eauto.
+    inv H.
+    rewrite inv_to_alg in H11.
+    rewrite <- has_enc_to_alg in H11; auto.
+    rewrite inv_to_alg in H2.
+    apply eq_sym in H2.
+    apply no_enc_eq in H2; auto; subst.
+    split; auto.
+    eapply CStmt_invp; eauto.
+  - exists cev.
+    exists ctr.
+    exists cus.
+    exists rs.
+    pose proof H6 as H.
+    apply ex_lookup in H6.
+    destruct H6.
+    erewrite lookup_ev in H; eauto.
+    inv H.
+    destruct x; simpl in H2; inv H2.
+    pose proof H10 as H.
+    apply ex_lookup in H10.
+    destruct H10.
+    erewrite lookup_ev in H; eauto.
+    inv H.
+    destruct x; simpl in H4; inv H4.
+    split; auto.
+    eapply CStmt_pub_namp; eauto.
+  - exists cev.
+    exists ctr.
+    exists cus.
+    exists rs.
+    pose proof H6 as H.
+    apply ex_lookup in H6.
+    destruct H6.
+    erewrite lookup_ev in H; eauto.
+    inv H.
+    destruct x; simpl in H2; inv H2.
+    pose proof H10 as H.
+    apply ex_lookup in H10.
+    destruct H10.
+    erewrite lookup_ev in H; eauto.
+    inv H.
+    destruct x; simpl in H4; inv H4.
+    split; auto.
+    eapply CStmt_priv_namp; eauto.
+  - exists cev.
+    exists ctr.
+    exists cus.
+    exists rs.
+    pose proof H7 as H.
+    apply ex_lookup in H7.
+    destruct H7.
+    erewrite lookup_ev in H; eauto.
+    inv H.
+    destruct x; simpl in H2; inv H2.
+    pose proof H11 as H.
+    apply ex_lookup in H11.
+    destruct H11.
+    erewrite lookup_ev in H; eauto.
+    inv H.
+    destruct x; simpl in H4; inv H4.
+    pose proof H15 as H.
+    apply ex_lookup in H15.
+    destruct H15.
+    erewrite lookup_ev in H; eauto.
+    inv H.
+    destruct x; simpl in H5; inv H5.
+    split; auto.
+    eapply CStmt_pub_nm2p; eauto.
+  - exists cev.
+    exists ctr.
+    exists cus.
+    exists rs.
+    pose proof H7 as H.
+    apply ex_lookup in H7.
+    destruct H7.
+    erewrite lookup_ev in H; eauto.
+    inv H.
+    destruct x; simpl in H2; inv H2.
+    pose proof H11 as H.
+    apply ex_lookup in H11.
+    destruct H11.
+    erewrite lookup_ev in H; eauto.
+    inv H.
+    destruct x; simpl in H4; inv H4.
+    pose proof H15 as H.
+    apply ex_lookup in H15.
+    destruct H15.
+    erewrite lookup_ev in H; eauto.
+    inv H.
+    destruct x; simpl in H5; inv H5.
+    split; auto.
+    eapply CStmt_priv_nm2p; eauto.
+Qed.
+
+(** So far, the proofs have been fairly straightforward.  But that
+    is all about to change.  The next step is to show that whenever
+    there are sequences of abstract state transitions, there are
+    corresponding sequences of transitions in the concrete semantics.
+    In the previous theorem, the transmitted term had to agree with
+    what was in the environment.  The challenge is to find a trace
+    that serves as a witness that has that property.
+
+    There is considerable freedom in the choice of received terms in
+    the trace of our witness.  The primary requirement is that when
+    randomness is removed, they agree with received terms in the
+    abstract trace.  Therefore, we choose received terms that have
+    zero as the randomness for any encryption within the term.
+
+    We also have to find a sequence of concrete fresh values that
+    corresponds to a sequence of abstract fresh values.  This is easy,
+    because fresh values are basic values and contain no encryptions
+    and so no randomness. *)
+
+(** Create a concrete term from an abstract term without randomness *)
+
+Fixpoint to_calg (x: alg): calg :=
+  match x with
+  | Tx v => CTx v
+  | Dt v => CDt v
+  | Nm v => CNm v
+  | Sk k => CSk k
+  | Ak k => CAk k
+  | Ik k => CIk k
+  | Ch v => CCh v
+  | Mg v => CMg v
+  | Tg z => CTg z
+  | Pr y z => CPr (to_calg y) (to_calg z)
+  | En y z => CEn 0 (to_calg y) (to_calg z)
+  | Hs y => CHs (to_calg y)
+  end.
+
+Lemma to_alg_calg:
+  forall val,
+    to_alg (to_calg val) = val.
+Proof.
+  induction val; simpl; auto.
+  - rewrite IHval1.
+    rewrite IHval2.
+    auto.
+  - rewrite IHval1.
+    rewrite IHval2.
+    auto.
+  - rewrite IHval.
+    auto.
+Qed.
+
+Lemma map_to_alg_calg:
+  forall xs,
+    map to_alg (map to_calg xs) = xs.
+Proof.
+  induction xs; simpl; auto.
+  rewrite to_alg_calg.
+  rewrite IHxs; auto.
+Qed.
+
+(** Concrete terms without encryptions have no randomness. *)
+
+Lemma to_calg_alg:
+  forall val,
+    chas_enc val = false ->
+    to_calg (to_alg val) = val.
+Proof.
+  induction val; intros; simpl in *; auto.
+  - rewrite orb_false_iff in H.
+    destruct H.
+    rewrite IHval1; auto.
+    rewrite IHval2; auto.
+  - inv H.
+  - rewrite IHval; auto.
+Qed.
+
+Lemma has_enc_lookup:
+  forall x cev v,
+    has_enc x = false ->
+    lookup v (to_env cev) = Some x ->
+    lookup v cev = Some (to_calg x).
+Proof.
+  intros.
+  pose proof H0 as G.
+  apply ex_lookup in H0.
+  destruct H0 as [y].
+  pose proof H0 as F.
+  apply lookup_ev in H0.
+  rewrite G in H0.
+  inv H0.
+  rewrite <- has_enc_to_alg in H.
+  rewrite to_calg_alg; auto.
+Qed.
+
+Definition to_cmaplet (m: var * alg): var * calg :=
+  let (v, x) := m in (v, to_calg x).
+
+(** Convert a concrete environment.  This is used to convert inputs to
+    a role.  Since they are basic values, they do not contain
+    randomness. *)
+
+Definition to_cenv (ev: env): cenv :=
+  map to_cmaplet ev.
+
+Lemma to_env_cenv:
+  forall ev,
+    to_env (to_cenv ev) = ev.
+Proof.
+  induction ev; simpl; auto.
+  rewrite IHev.
+  unfold to_cmaplet.
+  unfold to_maplet.
+  repeat expand_let_pairs; simpl.
+  rewrite to_alg_calg; auto.
+Qed.
+
+Lemma mk_env_cenv:
+  forall ds xs,
+    to_cenv (mk_env ds xs) = mk_cenv ds (map to_calg xs).
+Proof.
+  induction ds; intros; simpl; auto.
+  destruct a as [v s].
+  destruct xs as [|c xxs]; simpl; auto.
+  rewrite IHds.
+  auto.
+Qed.
+
+Lemma map_m_lookup_ev:
+  forall ev vs outs,
+    map_m (flip lookup (to_env ev)) vs = Some outs ->
+    exists couts,
+      map_m (flip lookup ev) vs = Some couts /\
+      map to_alg couts = outs.
+Proof.
+  intros ev vs.
+  revert ev.
+  induction vs; intros; simpl in *; auto.
+  - inv H.
+    exists []; simpl; auto.
+  - apply do_some in H.
+    destruct H as [x].
+    destruct H.
+    apply do_some in H0.
+    destruct H0 as [xs].
+    destruct H0.
+    inv H1.
+    apply IHvs in H0.
+    destruct H0 as [couts'].
+    destruct H0; subst.
+    pose proof H as G.
+    apply ex_lookup in H.
+    destruct H as [b].
+    exists (b :: couts').
+    unfold flip at 1.
+    rewrite H.
+    rewrite H0.
+    split; auto.
+    simpl.
+    unfold flip in G.
+    apply lookup_ev in H.
+    rewrite H in G.
+    inv G; subst; auto.
+Qed.
+
+(** Relate expressions
+
+<<
+   Parmeters:
+   cenv:      Input environment
+   list evt:  Input trace
+   list alg:  Input list of uniques
+   list nat:  Input list of random values
+   expr:      Expression code fragment
+   calg:      Value of the expression
+   list evt:  Output trace
+   list alg:  Output list of uniques
+   list nat:  Output list of random values
+   list cevt: Output added concrete events
+   list calg: Output added concrete uniques
+>>
+*)
+
+Inductive expr_sim:
+  cenv -> list evt -> list alg -> list nat -> expr ->
+  calg -> list evt -> list alg -> list nat ->
+  list cevt -> list calg -> Prop :=
+| Sim_quot: forall ev tr us rs x,
+    expr_sim ev tr us rs (Quot_ x) (CTg x)
+             tr us rs [] []
+| Sim_hash: forall ev tr us rs x a,
+    lookup x ev = Some a ->
+    expr_sim ev tr us rs (Hash_ x) (CHs a) tr us rs [] []
+| Sim_pair: forall ev tr us rs x y a b,
+    lookup x ev = Some a ->
+    lookup y ev = Some b ->
+    expr_sim ev tr us rs (Pair_ x y) (CPr a b) tr us rs [] []
+| Sim_encr_prob: forall ev tr us rs x y r a b,
+    lookup x ev = Some a ->
+    lookup y ev = Some b ->
+    expr_sim ev tr us (r :: rs) (Encr_ x y) (CEn r a b) tr us rs [] []
+| Sim_encr_zero: forall ev tr us x y a b,
+    lookup x ev = Some a ->
+    lookup y ev = Some b ->
+    expr_sim ev tr us [] (Encr_ x y) (CEn 0 a b) tr us [] [] []
+| Sim_frst: forall ev tr us rs x a b,
+    lookup x ev = Some (CPr a b) ->
+    expr_sim ev tr us rs (Frst_ x) a tr us rs [] []
+| Sim_scnd: forall ev tr us rs x a b,
+    lookup x ev = Some (CPr a b) ->
+    expr_sim ev tr us rs (Scnd_ x) b tr us rs [] []
+| Sim_decr: forall ev tr us rs x y r a b,
+    lookup x ev = Some (CEn r a b) ->
+    lookup y ev = Some (cinv b) ->
+    chas_enc (cinv b) = false ->
+    expr_sim ev tr us rs (Decr_ x y) a tr us rs [] []
+| Sim_frsh: forall ev tr us rs a,
+    expr_sim ev tr (a :: us) rs Frsh_ (to_calg a) tr us rs [] [to_calg a]
+| Sim_recv: forall ev tr us rs a c d,
+    lookup c ev = Some (CCh d) ->
+    expr_sim ev (Rv d a :: tr) us rs (Recv_ c) (to_calg a)
+             tr us rs [CRv d (to_calg a)] [].
+#[global]
+Hint Constructors expr_sim : core.
+
+Lemma expr_sim_to_alg:
+  forall cev tr us rs exp val tr' us' rs' dtr dus,
+    expr_sim cev tr us rs exp val tr' us' rs' dtr dus ->
+    map to_evt dtr ++ tr' = tr /\ map to_alg dus ++ us' = us.
+Proof.
+  intros.
+  destruct exp; inv H; simpl; auto;
+    rewrite to_alg_calg; auto.
+Qed.
+
+(** The simulation always exists *)
+
+Lemma expr_sem_expr_sim:
+  forall ev tr us exp val rs tr' us' cev,
+    expr_sem ev tr us exp val tr' us' ->
+    to_env cev = ev ->
+    exists cval rs' dtr dus,
+      expr_sim cev tr us rs exp cval tr' us' rs' dtr dus /\
+      to_alg cval = val.
+Proof.
+  intros.
+  destruct exp; inv H.
+  - exists (CTg s); exists rs; exists []; exists [].
+    auto.
+  - pose proof H5 as H.
+    apply ex_lookup in H5.
+    destruct H5.
+    erewrite lookup_ev in H; eauto.
+    inv H.
+    exists (CHs x); exists rs; exists []; exists [].
+    auto.
+  - pose proof H6 as H.
+    apply ex_lookup in H6.
+    destruct H6.
+    erewrite lookup_ev in H; eauto.
+    inv H.
+    pose proof H10 as H.
+    apply ex_lookup in H10.
+    destruct H10.
+    erewrite lookup_ev in H; eauto.
+    inv H.
+    exists (CPr x x0); exists rs; exists []; exists [].
+    auto.
+  - pose proof H6 as H.
+    apply ex_lookup in H6.
+    destruct H6.
+    erewrite lookup_ev in H; eauto.
+    inv H.
+    pose proof H10 as H.
+    apply ex_lookup in H10.
+    destruct H10.
+    erewrite lookup_ev in H; eauto.
+    inv H.
+    destruct rs as [| r rs].
+    + exists (CEn 0 x x0); exists []; exists []; exists [].
+      auto.
+    + exists (CEn r x x0); exists rs; exists []; exists [].
+      auto.
+  - pose proof H5 as H.
+    apply ex_lookup in H5.
+    destruct H5.
+    erewrite lookup_ev in H; eauto.
+    inv H.
+    destruct x; simpl in H2; inv H2.
+    exists x1; exists rs; exists []; exists [].
+    split; auto.
+    eapply Sim_frst; eauto.
+  - pose proof H5 as H.
+    apply ex_lookup in H5.
+    destruct H5.
+    erewrite lookup_ev in H; eauto.
+    inv H.
+    destruct x; simpl in H2; inv H2.
+    exists x2; exists rs; exists []; exists [].
+    split; auto.
+    eapply Sim_scnd; eauto.
+  - pose proof H3 as H.
+    apply ex_lookup in H3.
+    destruct H3.
+    erewrite lookup_ev in H; eauto.
+    inv H.
+    destruct x; simpl in H2; inv H2.
+    pose proof H7 as H.
+    apply ex_lookup in H7.
+    destruct H7.
+    erewrite lookup_ev in H; eauto.
+    inv H.
+    rewrite inv_to_alg in *.
+    apply eq_sym in H3.
+    rewrite <- has_enc_to_alg in H11.
+    apply no_enc_eq in H3; auto; subst.
+    exists x1; exists rs; exists []; exists [].
+    split; auto.
+    eapply Sim_decr; eauto.
+  - exists (to_calg val); exists rs; exists [];
+      exists [to_calg val].
+    rewrite to_alg_calg.
+    auto.
+  - pose proof H5 as H.
+    apply ex_lookup in H5.
+    destruct H5.
+    erewrite lookup_ev in H; eauto.
+    inv H.
+    destruct x; simpl in H2; inv H2.
+    exists (to_calg val); exists rs;
+      exists [CRv d (to_calg val)]; exists [].
+    rewrite to_alg_calg.
+    auto.
+Qed.
+
+Lemma expr_sim_injective:
+  forall cev tr us rs exp
+         val' tr' us' rs' dtr' cus'
+         val'' tr'' us'' rs'' dtr'' cus'',
+    expr_sim cev tr us rs exp val' tr' us' rs' dtr' cus' ->
+    expr_sim cev tr us rs exp val'' tr'' us'' rs'' dtr'' cus'' ->
+    val' = val'' /\ tr' = tr'' /\ us' = us'' /\
+    rs' = rs'' /\ dtr' = dtr'' /\ cus' = cus''.
+Proof.
+  intros.
+  destruct exp; inv H; inv H0; intuition.
+  - rewrite H5 in H6; inv H6; auto.
+  - rewrite H7 in H6; inv H6.
+    rewrite H15 in H14; inv H14; auto.
+  - rewrite H7 in H15; inv H15.
+    rewrite H16 in H14; inv H14; auto.
+  - rewrite H7 in H5; inv H5.
+    rewrite H6 in H14; inv H14; auto.
+  - rewrite H6 in H5; inv H5; auto.
+  - rewrite H6 in H5; inv H5; auto.
+  - rewrite H3 in H2; inv H2; auto.
+Qed.
+
+(** The desired simulation between abstract and concrete expressions *)
+
+Lemma expr_sem_sim_csem:
+  forall ev tr us exp val tr' us'
+         cev cval rs rs' dtr dus ctr cus,
+    expr_sem ev tr us exp val tr' us' ->
+    expr_sim cev tr us rs exp cval tr' us' rs' dtr dus ->
+    to_env cev = ev ->
+    to_alg cval = val ->
+    expr_csem cev (dtr ++ ctr) (dus ++ cus) rs exp cval ctr cus rs'.
+Proof.
+  intros.
+  pose proof H0 as G.
+  apply expr_sim_to_alg in H0.
+  destruct H0.
+  destruct exp; inv H; inv G; simpl; auto.
+  - eapply CExpr_frst; eauto.
+  - eapply CExpr_scnd; eauto.
+  - eapply CExpr_decr; eauto.
+Qed.
+
+(** Relate statements
+
+<<
+   Parmeters:
+   cenv:      Input environment
+   list evt:  Input trace
+   list alg:  Input list of uniques
+   list nat:  Input list of random values
+   stmt:      Statement
+   cenv:      Output environment
+   list evt:  Output trace
+   list alg:  Ouput list of uniques
+   list nat:  Output list of random values
+   list cevt: Output added concrete events
+   list calg: Output added concrete uniques
+>>
+*)
+
+Inductive stmt_sim:
+  cenv -> list evt -> list alg -> list nat -> stmt ->
+  cenv -> list evt -> list alg -> list nat ->
+  list cevt -> list calg -> Prop :=
+| Sim_bind: forall ev tr us rs v s exp val
+                   tr' us' rs' dtr dus,
+    expr_sim ev tr us rs exp val tr' us' rs' dtr dus ->
+    ctype_check s val ->
+    stmt_sim ev tr us rs (Bind (v, s) exp)
+             ((v, val) :: ev) tr' us' rs' dtr dus
+| Sim_send: forall ev tr us rs c x d a,
+    lookup c ev = Some (CCh d) ->
+    lookup x ev = Some a ->
+    stmt_sim ev (Sd d (to_alg a) :: tr) us rs
+             (Send c x) ev tr us rs [CSd d a] []
+| Sim_same: forall ev tr us rs x y,
+    stmt_sim ev tr us rs (Same x y) ev tr us rs [] []
+| Sim_ltkp: forall ev tr us rs x y z,
+    stmt_sim ev tr us rs (Ltkp x y z) ev tr us rs [] []
+| Sim_invp: forall ev tr us rs x y,
+    stmt_sim ev tr us rs (Invp x y) ev tr us rs [] []
+| Sim_namp: forall ev tr us rs x y,
+    stmt_sim ev tr us rs (Namp x y) ev tr us rs [] []
+| Sim_nm2p: forall ev tr us rs x y z,
+    stmt_sim ev tr us rs (Nm2p x y z) ev tr us rs [] [].
+#[global]
+Hint Constructors stmt_sim : core.
+
+Lemma stmt_sim_to_alg:
+  forall ev tr us rs stmt ev' tr' us' rs' dtr dus,
+    stmt_sim ev tr us rs stmt ev' tr' us' rs' dtr dus ->
+    map to_evt dtr ++ tr' = tr /\ map to_alg dus ++ us' = us.
+Proof.
+  intros.
+  destruct stmt; inv H; simpl; auto.
+  apply expr_sim_to_alg in H6; auto.
+Qed.
+
+(** The simulation always exists *)
+
+Lemma stmt_sem_stmt_sim:
+  forall cev ev tr us rs stmt ev' tr' us',
+    stmt_sem ev tr us stmt ev' tr' us' ->
+    to_env cev = ev ->
+    exists cev' rs' dtr dus,
+      stmt_sim cev tr us rs stmt cev' tr' us' rs' dtr dus /\
+      to_env cev' = ev'.
+Proof.
+  intros.
+  inv H.
+  - apply expr_sem_expr_sim
+      with (rs := rs)
+           (cev := cev) in H1; auto.
+    destruct H1 as [cval G].
+    destruct G as [rs' G].
+    destruct G as [dtr G].
+    destruct G as [dus G].
+    destruct G; subst.
+    rewrite <- type_check_equiv in H2.
+    exists ((v, cval) :: cev).
+    exists rs'.
+    exists dtr.
+    exists dus.
+    simpl.
+    split; auto.
+  - pose proof H2 as G.
+    apply ex_lookup in H2.
+    destruct H2 as [b].
+    pose proof H1 as F.
+    apply has_enc_lookup in H1; simpl; auto.
+    simpl in H1.
+    pose proof H as E.
+    apply lookup_ev in H.
+    rewrite H in G.
+    inv G.
+    exists cev.
+    exists rs.
+    exists [CSd d b].
+    exists [].
+    split; auto.
+  - pose proof H1 as G.
+    apply has_enc_lookup in H1; simpl; auto.
+    pose proof H2 as F.
+    apply has_enc_lookup in H2; simpl; auto.
+    exists cev.
+    exists rs.
+    exists [].
+    exists [].
+    split; auto.
+  - pose proof H1 as G.
+    apply has_enc_lookup in H1; simpl; auto.
+    pose proof H2 as F.
+    apply has_enc_lookup in H2; simpl; auto.
+    pose proof H3 as E.
+    apply has_enc_lookup in H3; simpl; auto.
+    exists cev.
+    exists rs.
+    exists [].
+    exists [].
+    split; auto.
+  - pose proof H1 as G.
+    apply has_enc_lookup in H1; simpl; auto.
+    rewrite inv_has_enc in H3.
+    pose proof H2 as F.
+    apply has_enc_lookup in H2; simpl; auto.
+    exists cev.
+    exists rs.
+    exists [].
+    exists [].
+    split; auto.
+  - pose proof H1 as G.
+    apply has_enc_lookup in H1; simpl; auto.
+    pose proof H2 as F.
+    apply has_enc_lookup in H2; simpl; auto.
+    exists cev.
+    exists rs.
+    exists [].
+    exists [].
+    split; auto.
+  - pose proof H1 as G.
+    apply has_enc_lookup in H1; simpl; auto.
+    pose proof H2 as F.
+    apply has_enc_lookup in H2; simpl; auto.
+    exists cev.
+    exists rs.
+    exists [].
+    exists [].
+    split; auto.
+  - pose proof H1 as G.
+    apply has_enc_lookup in H1; simpl; auto.
+    pose proof H2 as F.
+    apply has_enc_lookup in H2; simpl; auto.
+    pose proof H3 as E.
+    apply has_enc_lookup in H3; simpl; auto.
+    exists cev.
+    exists rs.
+    exists [].
+    exists [].
+    split; auto.
+  - pose proof H1 as G.
+    apply has_enc_lookup in H1; simpl; auto.
+    pose proof H2 as F.
+    apply has_enc_lookup in H2; simpl; auto.
+    pose proof H3 as E.
+    apply has_enc_lookup in H3; simpl; auto.
+    exists cev.
+    exists rs.
+    exists [].
+    exists [].
+    split; auto.
+Qed.
+
+Lemma stmt_sim_injective:
+  forall cev tr us rs stmt
+         cev' tr' us' rs' dtr' dus'
+         cev'' tr'' us'' rs'' dtr'' dus'',
+    stmt_sim cev tr us rs stmt cev' tr' us' rs' dtr' dus' ->
+    stmt_sim cev tr us rs stmt cev'' tr'' us'' rs'' dtr'' dus'' ->
+    cev' = cev'' /\ tr' = tr'' /\ us' = us'' /\
+    rs' = rs'' /\ dtr' = dtr'' /\ dus' = dus''.
+Proof.
+  intros.
+  destruct stmt; inv H; inv H0; intuition.
+  - eapply expr_sim_injective in H7; eauto.
+    repeat destruct_ex_and; subst; auto.
+  - eapply expr_sim_injective in H7; eauto.
+    repeat destruct_ex_and; subst; auto.
+  - eapply expr_sim_injective in H7; eauto.
+    repeat destruct_ex_and; subst; auto.
+  - eapply expr_sim_injective in H7; eauto.
+    repeat destruct_ex_and; subst; auto.
+  - eapply expr_sim_injective in H7; eauto.
+    repeat destruct_ex_and; subst; auto.
+  - eapply expr_sim_injective in H7; eauto.
+    repeat destruct_ex_and; subst; auto.
+  - rewrite H14 in H17.
+    inv H17; subst; auto.
+Qed.
+
+(** The desired simulation between abstract and concrete statements *)
+
+Lemma stmt_sem_sim_csem:
+  forall cev ev tr us rs stmt ev' tr' us'
+         cev' rs' dtr dus ctr cus,
+    stmt_sem ev tr us stmt ev' tr' us' ->
+    stmt_sim cev tr us rs stmt cev' tr' us' rs' dtr dus ->
+    to_env cev = ev ->
+    to_env cev' = ev' ->
+    stmt_csem cev (dtr ++ ctr) (dus ++ cus) rs stmt
+              cev' ctr cus rs'.
+Proof.
+  intros.
+  pose proof H0 as G.
+  apply stmt_sim_to_alg in H0.
+  destruct H0.
+  destruct stmt; inv H; inv G; simpl in *; subst; auto.
+  - inv H10.
+    eapply expr_sem_sim_csem in H15; eauto.
+  - apply has_enc_lookup in H6; auto.
+    apply has_enc_lookup in H7; auto.
+    eapply CStmt_same; eauto.
+    rewrite has_enc_to_alg.
+    rewrite to_alg_calg; auto.
+  - apply has_enc_lookup in H7; auto.
+    apply has_enc_lookup in H11; auto.
+    apply has_enc_lookup in H15; auto.
+    eapply CStmt_ltkp; eauto.
+  - apply has_enc_lookup in H6; auto.
+    pose proof H11 as G.
+    rewrite inv_has_enc in H11.
+    apply has_enc_lookup in H7; auto.
+    eapply CStmt_invp; eauto.
+    rewrite has_enc_to_alg.
+    rewrite to_alg_calg; auto.
+    destruct b; auto.
+  - apply has_enc_lookup in H6; auto.
+    apply has_enc_lookup in H10; auto.
+    eapply CStmt_pub_namp; eauto.
+  - apply has_enc_lookup in H6; auto.
+    apply has_enc_lookup in H10; auto.
+    eapply CStmt_priv_namp; eauto.
+  - apply has_enc_lookup in H7; auto.
+    apply has_enc_lookup in H11; auto.
+    apply has_enc_lookup in H15; auto.
+    eapply CStmt_pub_nm2p; eauto.
+  - apply has_enc_lookup in H7; auto.
+    apply has_enc_lookup in H11; auto.
+    apply has_enc_lookup in H15; auto.
+    eapply CStmt_priv_nm2p; eauto.
+Qed.
+
+(** Relate sequences of statements
+
+<<
+   Parmeters:
+   cenv:      Input environment
+   list evt:  Input trace
+   list alg:  Input list of uniques
+   list nat:  Input list of random values
+   list calg: Output list
+   list stmt: Statements
+   cenv:      Output environment
+   list nat:  Output list of random values
+   list cevt: Output added concrete events
+   list calg: Output added concrete uniques
+>>
+*)
+Inductive stmt_list_sim:
+  cenv -> list evt -> list alg -> list nat -> list calg -> list stmt ->
+  cenv -> list nat -> list cevt -> list calg -> Prop :=
+| Sim_return: forall ev rs outs vs,
+    map_m (flip lookup ev) vs = Some outs ->
+    stmt_list_sim ev [] [] rs outs [Return vs] ev rs [] []
+| Sim_stmts: forall ev tr us rs outs s stmts ev' tr' us' rs' dtr dus
+                    ev'' ctr cus rs'',
+    stmt_sim ev tr us rs s ev' tr' us' rs' dtr dus ->
+    stmt_list_sim ev' tr' us' rs' outs stmts ev'' rs'' ctr cus ->
+    stmt_list_sim ev tr us rs outs (s :: stmts)
+                  ev'' rs'' (dtr ++ ctr) (dus ++ cus).
+#[global]
+Hint Constructors stmt_list_sim : core.
+
+Lemma stmt_list_sim_to_alg:
+  forall stmts cev tr us rs couts cev' rs' ctr cus,
+    stmt_list_sim cev tr us rs couts stmts cev' rs' ctr cus ->
+    map to_evt ctr = tr /\ map to_alg cus = us.
+Proof.
+  induction stmts; intros; inv H; simpl; auto.
+  apply stmt_sim_to_alg in H7; auto.
+  destruct H7; subst.
+  apply IHstmts in H12.
+  destruct H12; subst.
+  repeat rewrite map_app; auto.
+Qed.
+
+(** The simulation always exists *)
+
+Lemma stmt_list_sem_stmt_list_sim:
+  forall stmts ev tr us rs outs ev' cev,
+    stmt_list_sem ev tr us outs stmts ev' ->
+    to_env cev = ev ->
+    exists couts cev' rs' ctr cus,
+      stmt_list_sim cev tr us rs couts stmts cev' rs' ctr cus /\
+      map to_alg couts = outs.
+Proof.
+  induction stmts; intros; simpl; auto; inv H.
+  - apply map_m_lookup_ev in H8.
+    destruct H8 as [couts].
+    destruct H; subst.
+    exists couts.
+    exists cev.
+    exists rs.
+    exists [].
+    exists [].
+    auto.
+  - pose proof H7 as H.
+    apply stmt_sem_stmt_sim
+      with (cev := cev) (rs := rs) in H7; auto.
+    destruct H7 as [cev' G].
+    destruct G as [rs' G].
+    destruct G as [dtr G].
+    destruct G as [dus G].
+    destruct G; subst.
+    pose proof H0 as F.
+    apply stmt_sim_to_alg in H0.
+    destruct H0; subst.
+    apply IHstmts
+      with (rs := rs') (cev := cev') in H9; auto.
+    destruct H9 as [couts G].
+    destruct G as [cev'' G].
+    destruct G as [rs'' G].
+    destruct G as [ctr G].
+    destruct G as [cus G].
+    exists couts.
+    exists cev''.
+    exists rs''.
+    exists (dtr ++ ctr).
+    exists (dus ++ cus).
+    destruct G; subst.
+    split; auto.
+    pose proof H0 as G.
+    apply stmt_list_sim_to_alg in H0.
+    destruct H0; subst.
+    eapply Sim_stmts in G; eauto.
+Qed.
+
+(** The desired simulation between abstract and concrete statement
+    sequences *)
+
+Lemma stmt_list_sem_sim_csem:
+  forall stmts ev tr us outs ev' cev rs
+         couts cev' ctr cus rs',
+    stmt_list_sem ev tr us outs stmts ev' ->
+    stmt_list_sim cev tr us rs couts stmts
+                  cev' rs' ctr cus ->
+    to_env cev = ev ->
+    map to_evt ctr = tr ->
+    map to_alg cus = us ->
+    stmt_list_csem cev ctr cus rs
+                   couts stmts cev' rs'.
+Proof.
+  induction stmts; intros; inv H; inv H0; simpl; auto.
+  - inv H9.
+  - pose proof H7 as G.
+    apply stmt_sim_to_alg in H7.
+    repeat rewrite map_app in H7.
+    destruct H7.
+    rewrite app_inv_head_iff in H; subst.
+    rewrite app_inv_head_iff in H0; subst.
+    pose proof H10 as F.
+    apply stmt_sem_stmt_sim
+      with (cev := cev) (rs := rs) in H10; auto.
+    destruct H10 as [cev'' D].
+    destruct D as [rs'' D].
+    destruct D as [dtr' D].
+    destruct D as [dus' D].
+    destruct D as [D]; subst.
+    eapply stmt_sim_injective in D; eauto.
+    repeat destruct_ex_and; subst.
+    eapply stmt_sem_sim_csem in G; eauto.
+Qed.
+
+Theorem stmt_list_sem_stmt_list_csem:
+  forall ev tr us outs stmts ev' cev rs,
+    stmt_list_sem ev tr us outs stmts ev' ->
+    to_env cev = ev ->
+    exists ctr cus couts cev' rs',
+      stmt_list_csem cev ctr cus rs couts stmts cev' rs' /\
+      map to_evt ctr = tr /\
+      map to_alg cus = us /\
+      map to_alg couts = outs.
+Proof.
+  intros.
+  pose proof H as G.
+  apply stmt_list_sem_stmt_list_sim
+    with (rs := rs) (cev := cev) in H; auto.
+  destruct H as [couts'].
+  destruct H as [cev'].
+  destruct H as [rs'].
+  destruct H as [ctr'].
+  destruct H as [cus'].
+  destruct H.
+  exists ctr'.
+  exists cus'.
+  exists couts'.
+  exists cev'.
+  exists rs'.
+  pose proof H as F.
+  apply stmt_list_sim_to_alg in F; auto.
+  destruct F.
+  eapply stmt_list_sem_sim_csem in H; eauto.
+Qed.
+
+Lemma ins_cins_inputs:
+  forall ds xs,
+    ins_inputs ds xs -> cins_inputs ds (map to_calg xs).
+Proof.
+  intros; induction H; simpl; auto.
+  apply CIns_inputs_pair; auto.
+  apply type_check_equiv.
+  rewrite to_alg_calg; auto.
+Qed.
+
+Theorem sem_csem_adequacy:
+  forall p ev rs e,
+    sem p ev e ->
+    exists cev,
+      csem p rs cev e.
+Proof.
+  intros.
+  unfold sem in H.
+  destruct H as [H G].
+  apply ins_cins_inputs in H.
+  apply stmt_list_sem_stmt_list_csem
+    with (cev := to_cenv (mk_env (ins p) (inputs e)))
+         (rs := rs) in G; auto.
+  - destruct G as [ctr G].
+    destruct G as [cus G].
+    destruct G as [couts G].
+    destruct G as [cev' G].
+    destruct G as [rs' G].
+    destruct G as [G F].
+    rewrite mk_env_cenv in G.
+    exists cev'.
+    unfold csem.
+    exists (map to_calg (inputs e)).
+    rewrite map_to_alg_calg.
+    split; auto.
+    split; auto.
+    exists ctr.
+    exists cus.
+    exists couts.
+    exists rs'.
+    split; auto.
+    intuition.
+  - rewrite to_env_cenv; auto.
+Qed.
+
+(** ** Alternate Concrete Execution Semantics
 
     In this semantics, the inputs are computed from the given output
     environment instead of being assumed to exist, and outputs are
@@ -561,7 +1834,7 @@ Definition csem' (p: proc) (rs: list nat) (cev: cenv) (e: role): Prop :=
     let ev_in := mk_cenv (ins p) cins in
     exists couts,
       mk_outs cev (body p) = Some couts /\
-      stmt_list_csem ev_in ctr cus rs couts (body p) cev [] [] rs' /\
+      stmt_list_csem ev_in ctr cus rs couts (body p) cev rs' /\
       outputs e = map to_alg couts.
 
 Theorem csem'_csem:
@@ -622,7 +1895,7 @@ Functional Scheme mk_outs_ind :=
 
 Lemma stmt_list_csem_outputs:
   forall ev tr us rs outs stmts ev' rs',
-    stmt_list_csem ev tr us rs outs stmts ev' [] [] rs' ->
+    stmt_list_csem ev tr us rs outs stmts ev' rs' ->
     mk_outs ev' stmts = Some outs.
 Proof.
   intros.
@@ -639,19 +1912,19 @@ Proof.
   - inv H.
     inv H7.
   - inv H.
-    apply IHo in H12; auto.
+    apply IHo in H10; auto.
   - inv H.
-    apply IHo in H12; auto.
+    apply IHo in H10; auto.
   - inv H.
-    apply IHo in H12; auto.
+    apply IHo in H10; auto.
   - inv H.
-    apply IHo in H12; auto.
+    apply IHo in H10; auto.
   - inv H.
-    apply IHo in H12; auto.
+    apply IHo in H10; auto.
   - inv H.
-    apply IHo in H12; auto.
+    apply IHo in H10; auto.
   - inv H.
-    apply IHo in H12; auto.
+    apply IHo in H10; auto.
 Qed.
 
 Theorem csem_csem':
